Fix bug caught by Paul

theories/BisimWeak.v
@@ -16,17 +16,63 @@ From CTree Require Import
 
 (* end hide *)
 
-Section Internal.
+(** Weak bisimulation of ctrees
 
-	(* We do not wish to observe internal non-deterministic choices.
-		We therefore want to consider states, i.e. ctrees, that can
-		be reached after a finite number of internal decisions, and
-		are such that they are ready to expose an observation: their
-		head constructor is either a Ret or a Vis.
-		*)
+  The relation [wbisim] captures an equivalence over [ctrees] akin to the traditional
+  weak bisimulation on process algebra.
+
+  Given the specific treatment that external events (Vis nodes in the tree) receive,
+  we explicitely distinguish two kind of challenges:
+
+  - Internal challenges correspond to a non-empty sequence of tau steps, and must be
+    matched by a possibly empty sequence of tau steps.
+    Transposed to the [ctree] formalism, this corresponds to crawling through 
+    as many [Choice] nodes as desired, but chosing specifically a _visible_ [Choice]
+    node to stop, and transit to any of the successor of this node.
+    The opponent then needs to find a way to answer similarly, but with the additional
+    possibility to stand still.
+
+    Electing a final node and picking one of its branches ensures that at least 
+    one tau step is taken, and any number of such internal steps can be taken before.
+    The distinction Visible/Invisible ensures we do not compare too finely the 
+    computations (i.e. (P + Q) + R cannot step to (P + R)).
+
+  - External challenges correspond to a non-tau step surrounded by arbitrary amounts 
+    of tau steps.
+    Transposed to the [ctree] formalism, this corresponds to:
+    + crawling through as many [Choice] nodes as desired until a Ret or Vis node is 
+      reached, let us call [t'] this new state
+    + having the opponent perform the same process up to a state [u']
+    + if [t'] and [u'] are related pure computations, we are good
+    + if [t'] and [u'] are Vis nodes of the same event, then they must match pointwise
+      a new internal challenge
+
+*)
+
+Section Stepping.
 
   Context {E : Type -> Type} {R : Type}.
 
+  (* External stepping
+    We have the following invariant: 
+    external t u -> t = Ret x \/ t = Vis e k
+  *)
+  Inductive external_ : ctree' E R -> ctree' E R -> Prop :=
+
+  | ExternalChoice {n} b (x : Fin.t n) k t :
+    		external_ (observe (k x)) t ->
+    		external_ (ChoiceF b n k) t
+
+  | ExternalRet x :
+    		external_ (RetF x) (RetF x)
+
+  | ExternalVis {X} (e : E X) k k' :
+    		(forall x, k x ≅ k' x) -> (* Because [external_] stops right there, we need to close explicitly up to [equ] if we want to be stable under it *)
+    		external_ (VisF e k) (VisF e k').
+
+  Definition external u v := external_ (observe u) (observe v).
+
+  (* Internal stepping *)
   Inductive internal_ : ctree' E R -> ctree' E R -> Prop :=
 
   | InternalStep b {n} (x : Fin.t n) k t :
@@ -39,11 +85,16 @@ Section Internal.
 
   Definition internal u v := internal_ (observe u) (observe v).
 
-  Variant internal_refl : ctree E R -> ctree E R -> Prop :=
-  | InternalRefl : forall u, internal_refl u u 
-  | InternalRel  : forall u v, internal u v -> internal_refl u v.
+  (* Reflexive closure of the internal stepping *)
+  Variant refl_clo {X} (R : X -> X -> Prop): X -> X -> Prop :=
+  | ReflCloRefl : forall u, refl_clo R u u 
+  | ReflCloRel  : forall u v, R u v -> refl_clo R u v.
 
-End Internal.
+  Definition internal_refl := refl_clo internal. 
+
+End Stepping.
+#[global] Hint Constructors refl_clo: core.
+#[global] Hint Unfold internal_refl : core.
 
 Section wbisim.
 
@@ -55,29 +106,35 @@ Section wbisim.
 	bisimulation world to ensuring that they can take a small step
 	emmitting the same event. *)
 
-  Variant matchingL (bisim : ctree E R1 -> ctree E R2 -> Prop) :
-    ctree E R1 -> ctree E R2 -> Prop :=
+  Variant matchingL_ (bisim : ctree E R1 -> ctree E R2 -> Prop) :
+    ctree' E R1 -> ctree' E R2 -> Prop :=
   | MatchLRet x y (RET : RR x y) :
-     matchingL bisim (Ret x) (Ret y)
+     matchingL_ bisim (RetF x) (RetF y)
   | MatchLVis {X} (e : E X) k1 k2 
      (RET : forall v t', 
         internal_refl (k1 v) t' ->
         exists u', internal_refl (k2 v) u' /\ bisim t' u'):
-     matchingL bisim (Vis e k1) (Vis e k2)
+     matchingL_ bisim (VisF e k1) (VisF e k2)
   . 
-  Hint Constructors matchingL: core.
+  Hint Constructors matchingL_ : core.
+  Definition matchingL bisim u v := matchingL_ bisim (observe u) (observe v).
 
-  Variant matchingR (bisim : ctree E R1 -> ctree E R2 -> Prop) :
-    ctree E R1 -> ctree E R2 -> Prop :=
+  Variant matchingR_ (bisim : ctree E R1 -> ctree E R2 -> Prop) :
+    ctree' E R1 -> ctree' E R2 -> Prop :=
   | MatchRRet x y (RET : RR x y) :
-     matchingR bisim (Ret x) (Ret y)
+     matchingR_ bisim (RetF x) (RetF y)
   | MatchRVis {X} (e : E X) k1 k2 
      (RET : forall v t', 
-        internal_refl (k1 v) t' ->
-        exists u', internal_refl (k2 v) u' /\ bisim t' u'):
-     matchingR bisim (Vis e k1) (Vis e k2)
+        internal_refl (k2 v) t' ->
+        exists u', internal_refl (k1 v) u' /\ bisim t' u'):
+     matchingR_ bisim (VisF e k1) (VisF e k2)
   . 
-  Hint Constructors matchingR: core.
+  Hint Constructors matchingR_ : core.
+
+  (* step_vis : ctree E X -> {Y : Type & e : E Y & v : Y} -> ctree E X -> Prop 
+    Does this lead to exactly the same thing?
+  *)
+  Definition matchingR bisim u v := matchingR_ bisim (observe u) (observe v).
 
   Variant wbisimF (wbisim : ctree E R1 -> ctree E R2 -> Prop) :
     ctree E R1 -> ctree E R2 -> Prop :=
@@ -87,23 +144,21 @@ Section wbisim.
               exists t', internal_refl t t' /\ wbisim u' t')
             (SIMBI : forall t', internal t t' ->
               exists u', internal_refl u u' /\ wbisim u' t')
-            (SIMFE : forall u', schedule u u' ->
-              exists t', schedule t t' /\ matchingL wbisim u' t')
-            (SIMBE : forall t', schedule t t' ->
-              exists u', schedule u u' /\ matchingR wbisim u' t')
+            (SIMFE : forall u', external u u' ->
+              exists t', external t t' /\ matchingL wbisim u' t')
+            (SIMBE : forall t', external t t' ->
+              exists u', external u u' /\ matchingR wbisim u' t')
                :
       wbisimF wbisim u t.
  
   Hint Constructors wbisimF: core.
-(* 
-  Definition wbisim_ eq : ctree E R1 -> ctree E R2 -> Prop :=
-	fun t1 t2 => bisimF eq (observe t1) (observe t2). *)
 
   Lemma matchingL_mono u v sim sim'
               (IN : matchingL sim u v)
               (LE : sim <= sim') :
         matchingL sim' u v.
   Proof.
+    unfold matchingL in *.
     inv IN; auto. constructor; intros. edestruct RET as (? & ? & ?); eauto.
     eexists; split; eauto. 
     apply LE; auto.
@@ -115,12 +170,12 @@ Section wbisim.
               (LE : sim <= sim') :
         matchingR sim' u v.
   Proof.
+    unfold matchingR in *.
     inv IN; auto. constructor; intros. edestruct RET as (? & ? & ?); eauto.
     eexists; split; eauto. 
     apply LE; auto.
   Qed.
   Hint Resolve matchingR_mono: core.
-
 
   Program Definition fwbisim : mon (ctree E R1 -> ctree E R2 -> Prop) := {| body := wbisimF |}.
   Next Obligation.
@@ -150,5 +205,190 @@ Notation "x [≊] y" := (bt_bis eq _ x y) (at level 79).
 
 Arguments wbisim _ _ _ _/.
 #[global] Hint Constructors wbisimF: core.
-#[global] Hint Constructors matchingL: core.
-#[global] Hint Constructors matchingR: core.
+#[global] Hint Constructors matchingL_: core.
+#[global] Hint Constructors matchingR_: core.
+
+Lemma external_active_ : forall {E R} (t u : ctree' E R),
+  external_ t u ->
+  active_ u.
+Proof.
+  intros * INTERN. 
+  now induction INTERN.
+Qed.
+
+Lemma external_active : forall {E R} (t u : ctree E R),
+  external t u ->
+  active u.
+Proof.
+  intros * SCHED; red.
+  now induction SCHED.
+Qed.
+
+Lemma matchingL_active_refl {E R} (RR : R -> R -> Prop)
+  (eq : ctree E R -> ctree E R -> Prop) (t : ctree E R)
+  `{Reflexive _ RR} `{Reflexive _ eq} :
+  active t ->
+  matchingL RR eq t t.
+Proof. 
+  unfold matchingL; intros []; eauto.
+Qed.
+
+Lemma matchingR_active_refl {E R} (RR : R -> R -> Prop)
+  (eq : ctree E R -> ctree E R -> Prop) (t : ctree E R)
+  `{Reflexive _ RR} `{Reflexive _ eq} :
+  active t ->
+  matchingR RR eq t t.
+Proof. 
+  unfold matchingR; intros []; eauto.
+Qed.
+
+(*
+Lemma matchingL_active_sym {E R} (RR : R -> R -> Prop)
+   (eq : ctree E R -> ctree E R -> Prop) (t u : ctree E R)
+   `{Symmetric _ RR} :
+   matchingR RR eq t u ->
+   matchingL RR (converse eq) u t.
+Proof.
+  unfold matchingL, matchingR; intros []; eauto.
+  constructor; intros. 
+  edestruct RET as (? & ? & ?); eauto.
+Qed.
+
+Lemma matchingR_active_sym {E R} (RR : R -> R -> Prop)
+   (eq : ctree E R -> ctree E R -> Prop) (t u : ctree E R)
+   `{Symmetric _ RR} :
+   matchingR RR eq t u ->
+   matchingR RR (converse eq) u t.
+Proof.
+  unfold matchingR; intros []; eauto.
+Qed. *)
+
+Lemma matching_active_sym {E R} (RR : R -> R -> Prop)
+   (eq : ctree E R -> ctree E R -> Prop) (t u : ctree' E R)
+   `{Symmetric _ RR} :
+   matching RR eq t u ->
+   matching RR (converse eq) u t.
+Proof.
+  intros []; auto.
+Qed.
+
+Section wbisim_equiv.
+
+	Variable (E : Type -> Type) (R : Type) (RR : R -> R -> Prop).
+  Notation T  := (coinduction.T (fwbisim (E := E) RR)).
+  Notation t  := (coinduction.t (fwbisim (E := E) RR)).
+	Notation bt := (coinduction.bt (fwbisim (E := E) RR)).
+
+
+  (** [eq] is a post-fixpoint, thus [const eq] is below [t] *)
+	Lemma refl_t {RRR: Reflexive RR}: const eq <= t.
+	Proof.
+    apply leq_t.
+		intros p t ? <-. cbn.
+    constructor; eauto.
+    - intros t' SCHED; eauto.
+      exists t'; split; auto.
+      apply matchingL_active_refl; auto.
+      eapply external_active; eauto.
+    - intros t' SCHED.
+      exists t'; split; auto.
+      apply matchingR_active_refl; auto.
+      eapply external_active; eauto.
+	Qed.
+
+(*
+	(** converse is compatible *)
+	Lemma converse_t {RRS: Symmetric RR}: converse <= t.
+	Proof.
+		apply leq_t. intros S t u H; cbn in *.
+    destruct H. constructor; eauto.
+    - intros t' SCHED.
+      edestruct SIMBE as (u' & SCHED' & MATCH'); eauto.
+      edestruct SIMFE as (t'' & SCHED'' & MATCH''); eauto.
+      exists u'; split; auto.
+      apply matching_active_sym; auto.
+    - intros u' SCHED.
+      edestruct SIMF as (t' & SCHED' & MATCH'); eauto.
+      exists t'; split; auto.
+      apply matching_active_sym; auto.
+	Qed.
+
+	(** thus wbisimilarity, [t R], [b (t R)] and [T f R] are always reflexive relations *)
+	#[global] Instance Reflexive_t `{Reflexive _ RR} S: Reflexive (t S).
+	Proof.  intro. now apply (ft_t refl_t). Qed.
+	#[global] Instance Reflexive_T `{Reflexive _ RR} f S: Reflexive (T f S).
+	Proof.  intro. now apply (fT_T refl_t). Qed.
+	#[global] Instance Reflexive_bt `{Reflexive _ RR} S: Reflexive (bt S).
+	Proof.  intro. now apply (fbt_bt refl_t). Qed.
+
+	(** thus wbisimilarity, [t R], [b (t R)] and [T f R] are always symmetric relations *)
+	#[global] Instance Symmetric_t `{Symmetric _ RR} S: Symmetric (t S).
+	Proof.  intros ???. now apply (ft_t converse_t). Qed.
+	#[global] Instance Symmetric_T `{Symmetric _ RR} f S: Symmetric (T f S).
+	Proof.  intros ???. now apply (fT_T converse_t). Qed.
+	#[global] Instance Symmetric_bt `{Symmetric _ RR} S: Symmetric (bt S).
+	Proof.  intros ???. now apply (fbt_bt converse_t). Qed.
+
+End wbisim_equiv.
+
+#[global] Instance wbisim_trans {E R}: Transitive (@wbisim E R).
+Proof.
+  red. unfold wbisim. coinduction S IH.
+  intros t u v eq1 eq2.
+  step in eq1; step in eq2.
+  inversion eq1 as [? ? SIMF1 SIMB1]; subst.
+  inversion eq2 as [? ? SIMF2 SIMB2]; subst.
+  constructor.
+  - intros u' SCHED.
+    apply SIMF1 in SCHED as (ou' & SCHEDu & MATCHut).
+    apply SIMF2 in SCHEDu as (ov' & SCHEDv & MATCHvu).
+    exists ov'; split; auto.
+    inv MATCHvu.
+    + inv MATCHut; auto.
+    + inv MATCHut.
+      dependent induction H3.
+      constructor.
+      intros ?.
+      eapply IH; eauto.
+  - intros t' SCHED.
+    apply SIMB2 in SCHED as (ou' & SCHEDu & MATCHut).
+    apply SIMB1 in SCHEDu as (ov' & SCHEDv & MATCHvu).
+    exists ov'; split; auto.
+    inv MATCHvu.
+    + inv MATCHut; auto.
+    + inv MATCHut.
+      dependent induction H2.
+      constructor.
+      intros ?.
+      eapply IH; eauto.
+Qed.
+
+#[global] Instance equ_schedule {E X}:
+	Proper (equ eq ==> equ eq ==> iff) (@schedule E X).
+Proof.
+  repeat red; intros * EQ1 * EQ2; split; intros SCHED.
+  - step in EQ1; step in EQ2.
+    unfold schedule in *.
+    hinduction SCHED before X.
+    + intros. inv EQ1. apply inj_pair2 in H2. subst.
+      eapply SchedChoice with x1.
+      apply IHSCHED. specialize (REL x1).
+      step in REL. apply REL. auto.
+    + intros. inv EQ1; inv EQ2; constructor.
+    + intros. inv EQ1. inv EQ2. apply inj_pair2 in H2, H3, H5, H6. subst.
+      constructor. intros.
+      rewrite <- REL0, <- REL. auto.
+  - step in EQ1; step in EQ2.
+    unfold schedule in *.
+    hinduction SCHED before X.
+    + intros. inv EQ1. apply inj_pair2 in H3. subst.
+      eapply SchedChoice with x.
+      apply IHSCHED. specialize (REL x).
+      step in REL. apply REL. auto.
+    + intros. inv EQ1; inv EQ2; constructor.
+    + intros. inv EQ1. inv EQ2. apply inj_pair2 in H3, H4, H6, H7. subst.
+      constructor. intros.
+      rewrite REL0, REL. auto.
+Qed.
+
+*)
